---
title: "Methods Homework 8"
author: "Tim Vigers"
date: "`r format(Sys.time(), '%d %B %Y')`"
output: pdf_document
---

```{r setup, include=FALSE}
knitr::opts_chunk$set(echo = TRUE)
```

#1. Show that SSTotal = SSModel + SSError
$$
SS_\text{Total} = \sum_{i=1}^n(Y_i-\bar{Y})^2=\sum_{i=1}^n((Y_i-\hat{Y}_i)+(\hat{Y}_i-\bar{Y}))^2=
$$
$$
\sum_{i=1}^n(Y_i-\hat{Y}_i)^2+\sum_{i=1}^n(\hat{Y}_i-\bar{Y})^2+2\sum_{i=1}^n(Y_i-\hat{Y}_i)(\hat{Y}_i-\bar{Y})
$$
$$
\text{From the lecture notes we know that:}
$$
$$
SS_\text{Error}=\sum_{i=1}^n(Y_i-\hat{Y}_i)^2
\text{ and }SS_\text{Model}=\sum_{i=1}^n(\hat{Y}_i-\bar{Y})^2
$$
$$
\text{So: }
$$
$$
SS_\text{Total} = SS_\text{Error} + SS_\text{Model} + 2\sum_{i=1}^n(Y_i-\hat{Y}_i)(\hat{Y}_i-\bar{Y})
$$
$$
2\sum_{i=1}^n(Y_i-\hat{Y}_i)(\hat{Y}_i-\bar{Y}) =
$$
$$
2\sum_{i=1}^nY_i\hat{Y}_i-\bar{Y}Y_i-\hat{Y}_i^2+\bar{Y}\hat{Y}_i
$$
$$
\text{This can be rearranged to:}
$$
$$
2(\sum_{i=1}^n\hat{Y}_i(Y_i-\hat{Y}_i)-\bar{Y}(Y_i-\hat{Y}_i))=2(\sum_{i=1}^n\hat{Y}_i(Y_i-\hat{Y}_i)-\sum_{i=1}^n\bar{Y}(Y_i-\hat{Y}_i))
$$
$$
\bar{Y}\text{ is a constant, so it can be pulled out of the sum, meaning: }
$$
$$
\sum_{i=1}^n\bar{Y}(Y_i-\hat{Y}_i) = \bar{Y}\sum_{i=1}^n(Y_i-\hat{Y}_i)=\bar{Y}*0 = 0
$$
$$
\text{Because }\hat{Y_i}=\hat{\beta}_0+\hat{\beta}_1X_i\text{ :}
$$
$$
\sum_{i=1}^n\hat{Y}_i(Y_i-\hat{Y}_i) = \sum_{i=1}^n(\hat{\beta}_0+\hat{\beta}_1X_i)(Y_i-\hat{Y}_i) = \hat{\beta}_0\sum_{i=1}^n(Y_i-\hat{Y}_i)+\hat{\beta}_1\sum_{i=1}^nX_i(Y_i-\hat{Y}_i)
$$
$$
\text{As before, we've pulled out the constants and know both of the above sums are equal to 0. Therefore: }
$$
$$
2\sum_{i=1}^n(Y_i-\hat{Y}_i)(\hat{Y}_i-\bar{Y}) = 2 (0+0-0) = 0
$$
$$
\text{Which leaves us with: }
$$
$$
SS_\text{Total} = SS_\text{Error} + SS_\text{Model} + 0
$$